
\documentclass[12pt]{article}
\usepackage{amsmath}
\usepackage{amssymb}
\usepackage{amsthm}
\usepackage{amsfonts}
\usepackage{graphicx}
\usepackage{textcomp}
\usepackage{hyperref}
\usepackage{tikz}
\usepackage{enumitem}
\usepackage{mathtools}
\usepackage{float}
\usepackage{cleveref}
\usepackage{hyperref}
\usepackage{csquotes}

\begin{document}

\title{MACM 101 Chapter 1 Homework}
\author{Alexander Ng}
\date{Monday, September 30, 2024}

\maketitle 

\subsection*{Question 4}

\subsubsection*{Part a}

\[
\begin{array}{|c|c|c|c|c|c|c|c|}
\hline
p & q & r & p \lor q & q \lor r & (p \lor q) \lor r & p \lor (q \lor r) \\
\hline
1 & 1 & 1 & 1 & 1 & 1 & 1 \\
1 & 1 & 0 & 1 & 1 & 1 & 1 \\
1 & 0 & 1 & 1 & 1 & 1 & 1 \\
1 & 0 & 0 & 1 & 0 & 1 & 1 \\
0 & 1 & 1 & 1 & 1 & 1 & 1 \\
0 & 1 & 0 & 1 & 1 & 1 & 1 \\
0 & 0 & 1 & 0 & 1 & 1 & 1 \\
0 & 0 & 0 & 0 & 0 & 0 & 0 \\
\hline
\end{array}
\]

\subsubsection*{Part b}

\[
\begin{array}{|c|c|c|c|c|c|c|c|}
\hline
p & q & r & p \land q & q \land r & (p \land q) \land r & p \land (q \land r) \\
\hline
1 & 1 & 1 & 1 & 1 & 1 & 1 \\
1 & 1 & 0 & 1 & 0 & 0 & 0 \\
1 & 0 & 1 & 0 & 0 & 0 & 0 \\
1 & 0 & 0 & 0 & 0 & 0 & 0 \\
0 & 1 & 1 & 0 & 1 & 0 & 0 \\
0 & 1 & 0 & 0 & 0 & 0 & 0 \\
0 & 0 & 1 & 0 & 0 & 0 & 0 \\
0 & 0 & 0 & 0 & 0 & 0 & 0 \\
\hline
\end{array}
\]

\subsection*{Question 12}

\subsubsection*{Part a}

\[
\begin{array}{|c|c|c|c|c|c|c|c|}
\hline
p & q & p \lor q & \neg p & \neg p \land (p \lor q) & [\neg p \land (p \lor q)] \to q \\
\hline
1 & 1 & 1 & 0 & 0 & 1 \\
1 & 0 & 1 & 0 & 0 & 1 \\
0 & 1 & 1 & 1 & 1 & 1 \\
0 & 0 & 0 & 1 & 0 & 1 \\
\hline
\end{array}
\]

\subsubsection*{Part b}

\[
\begin{array}{|c|c|c|c|c|c|c|c|}
\hline
p & q & r & p \to q & q \to r & (p \to q) \land (q \to r) & p \to r & [(p \to q) \land (q \to r)] \to (p \to r) \\
\hline
1 & 1 & 1 & 1 & 1 & 1 & 1 & 1 \\
1 & 1 & 0 & 1 & 0 & 0 & 0 & 1 \\
1 & 0 & 1 & 0 & 1 & 0 & 1 & 1 \\
1 & 0 & 0 & 0 & 1 & 0 & 0 & 1 \\
0 & 1 & 1 & 1 & 1 & 1 & 1 & 1 \\
0 & 1 & 0 & 1 & 0 & 0 & 1 & 1 \\
0 & 0 & 1 & 1 & 1 & 1 & 1 & 1 \\
0 & 0 & 0 & 1 & 1 & 1 & 1 & 1 \\
\hline
\end{array}
\]

\subsubsection*{Part c}

\[
\begin{array}{|c|c|c|c|c|c|}
\hline
p & q & p \to q & p \land (p \to q) & [p \land (p \to q)] \to q \\
\hline
1 & 1 & 1 & 1 & 1 \\
1 & 0 & 0 & 0 & 1 \\
0 & 1 & 1 & 0 & 1 \\
0 & 0 & 1 & 0 & 1 \\
\hline
\end{array}
\]

\subsubsection*{Part d}

\[
\begin{array}{|c|c|c|c|c|c|c|c|c|}
\hline
p & q & r & p \lor q & p \to r & q \to r & (p \lor q) \land (p \to r) & (p \lor q) \land (p \to r) \land (q \to r) & [(p \lor q) \land (p \to r) \land (q \to r)] \to r \\
\hline
1 & 1 & 1 & 1 & 1 & 1 & 1 & 1 & 1 \\
1 & 1 & 0 & 1 & 0 & 0 & 0 & 0 & 1 \\
1 & 0 & 1 & 1 & 1 & 1 & 1 & 1 & 1 \\
1 & 0 & 0 & 1 & 0 & 1 & 0 & 0 & 1 \\
0 & 1 & 1 & 1 & 1 & 1 & 1 & 1 & 1 \\
0 & 1 & 0 & 1 & 0 & 0 & 0 & 0 & 1 \\
0 & 0 & 1 & 0 & 1 & 1 & 0 & 0 & 1 \\
0 & 0 & 0 & 0 & 0 & 1 & 0 & 0 & 1 \\
\hline
\end{array}
\]

\subsection*{Question 14}

\subsubsection*{Part a}

\[
\neg p \land (p \lor q) \to q
\]

$p \to q$ is false when $p$ is true and $q$ is false.

Assume $ \neg p \land (p \lor q)$ is true.

When $ \neg p \land (p \lor q)$ is true, then both $ \neg p$ and $ p \lor q$ are true.

When $ \neg p$ is true, then $ p$ is false.

When $ p \lor q$ is true with $ p$ false, then we require that $ q$
is true, and thus $ \neg p \land (p \lor q) \to q$ is always true
(as we know that the conditional statement is also true whenever
$ \neg p \land (p \lor q)$ is false). This implies that
$ \neg p \land (p \lor q) \to q \equiv \mathbb{T}$.

\subsubsection*{Part b}

\[
[(p \to q) \land (q \to r)] \to (p \to r)
\]

$p \to q$ is false when $p$ is true and $q$ is false.

Assume $(p \to q) \land (q \to r)$ is true.

When $(p \to q) \land (q \to r)$ is true, then both
$p \to q$ and $q \to r$ are true.

When $p$ is true, because $p \to q$ is true, $q$ must also be true, and
because $q \to r$ is true, $r$ must also be true. $p \to r$ is also true
when both $p$ and $r$ are true.

When $p$ is false, then $p \to r$ is true as well.

Therefore, $p \to r$ is true in each case, and thus
$[(p \to q) \land (q \to r)] \to (p \to r)$ is
always true (as we know that the conditional statement is also true whenever
$(p \to q) \land (q \to r)$ is false).

This implies that
$[(p \to q) \land (q \to r)] \to (p \to r) \equiv \mathbb{T} $ 

\subsubsection*{Part c}

\[
p \land (p \to q) \to q
\]

$p \to q$ is false when $p$ is true and $q$ is false.

Assume $p \land (p \to q)$ is true.

When $p \land (p \to q)$ is true, both $p$ and $p \to q$ are true.

When $p \to q$ and $p$ are both true, we also require that $q$ is true. 
Thus, $p \land (p \to q) \to q$ is always true (since we know the conditional 
statement is also true whenever $p \land (p \to q)$ is false). 

This implies that $p \land (p \to q) \to q \equiv \mathbb{T} $

\subsubsection*{Part d}

\[
[(p \lor q) \land (p \to r) \land (q \to r)] \to r
\]

$p \to q$ is false when $p$ is true and $q$ is false.

Assume $(p \lor q) \land (p \to r) \land (q \to r)$ is true.

When $(p \lor q) \land (p \to r) \land (q \to r)$ is true, then $p \lor q$, 
$p \to r$, and $q \to r$ are all true.

$p \lor q$ being true implies that either $p$ or $q$ is true.

When $p$ is true, then $r$ is true as well (since $p \to r$ is true).

When $q$ is true, then $r$ is true as well (since $q \to r$ is true).

However, $r$ is true in each case, and thus 
$[(p \lor q) \land (p \to r) \land (q \to r)] \to r$ is always true 
(as we know that the conditional statement is also true whenever 
$(p \lor q) \land (p \to r) \land (q \to r)$ is false). This then gives us that

\[
[(p \lor q) \land (p \to r) \land (q \to r)] \to r \equiv \mathbb{T}
\]

\subsection*{Question 22}

Show that $p \to q$ and $\neg q \to \neg p$ are logically equivalent.

\begin{enumerate}
  \item $p \to q \equiv \neg p \lor q$ (Logical Equivalences)
  \item $\equiv \neg p \lor \neg \neg q$ (Double Negation Law)
  \item $\equiv \neg \neg q \lor \neg p$ (Commutative Law)
  \item $\equiv \neg q \to \neg p$ (Logical Equivalences)
  \item $\therefore p \to q \equiv \neg q \to \neg p$
\end{enumerate}

\subsection*{Question 24}

Show that $\neg (p \oplus q)$ and $p \leftrightarrow q$ are logically equivalent.


\begin{enumerate}
  \item $\neg (p \oplus q) \equiv \neg ((p \lor q) \land (\neg p \lor \neg q))$ (Definition)
  \item $\equiv \neg [(p \land (\neg p \lor \neg q)) \lor (q \land (\neg p \lor \neg q))]$ (Distributive Law)
  \item $\equiv \neg [((p \land \neg p) \lor (p \land \neg q)) \lor ((q \land \neg p) \lor (q \land \neg q))]$ (Distributive Law)
  \item $\equiv \neg [(\mathbb{F} \lor (p \land \neg q)) \lor ((q \land \neg p) \lor \mathbb{F})]$ By $p \land \neg p \equiv \mathbb{F}$
  \item $\equiv \neg [(p \land \neg q) \lor (q \land \neg p)]$ (Identity Law)
  \item $\equiv \neg (p \land \neg q) \land \neg (q \land \neg p)$ (De Morgan's Law)
  \item $\equiv (\neg p \lor q) \land (\neg q \lor p)$ (De Morgan's Law and Double Negation Law)
  \item $\equiv (p \to q) \land (q \to p)$ (Logical Equivalence)
  \item $\equiv p \leftrightarrow q$ (Logical Equivalence)
\end{enumerate}

\subsection*{Question 40}

$s^* = s$ if the compound proposition can be simplified to a variable or the
negation of a variable

\subsection*{Question 46}

Not sure how to do this one.

\end{document}
